

Tutorial-2

$$\Rightarrow \underline{\underline{a}} \cdot (\underline{\underline{b}} \wedge \underline{\underline{A}}) = (\underline{\underline{a}} \wedge \underline{\underline{b}}) \cdot \underline{\underline{A}}$$

$$\begin{aligned} & a_i \underline{\underline{\delta}}_i \cdot (b_j \underline{\underline{\delta}}_j \wedge A_{p2} \underline{\underline{\delta}}_p \underline{\underline{\delta}}_2) \\ &= a_i \underline{\underline{\delta}}_i \cdot (b_j A_{p2} \varepsilon_{kjp} \underline{\underline{\delta}}_k \underline{\underline{\delta}}_2) \\ &= a_i b_j A_{p2} \varepsilon_{kjp} \underline{\underline{\delta}}_2 (\underline{\underline{\delta}}_i \cdot \underline{\underline{\delta}}_k) \\ &= a_i b_j A_{p2} \varepsilon_{kjp} \underline{\underline{\delta}}_2 \delta_{ik} = a_i b_j A_{p2} \varepsilon_{ijp} \underline{\underline{\delta}}_2 \end{aligned}$$

$$\begin{aligned} (\underline{\underline{a}} \wedge \underline{\underline{b}}) \cdot \underline{\underline{A}} &= (a_i \underline{\underline{\delta}}_i \wedge b_j \underline{\underline{\delta}}_j) \cdot A_{p2} \underline{\underline{\delta}}_p \underline{\underline{\delta}}_2 \\ &= a_i b_j \varepsilon_{ijk} \underline{\underline{\delta}}_k \cdot A_{p2} \underline{\underline{\delta}}_p \underline{\underline{\delta}}_2 \\ &= a_i b_j \varepsilon_{ijk} A_{p2} \underline{\underline{\delta}}_2 (\underline{\underline{\delta}}_k \cdot \underline{\underline{\delta}}_p) \\ &= a_i b_j \varepsilon_{ijk} A_{p2} \delta_{kp} \underline{\underline{\delta}}_2 \\ &= a_i b_j \varepsilon_{ijk} A_{k2} \underline{\underline{\delta}}_2 \end{aligned}$$

$$2) (a \wedge b) \cdot (a \wedge b) + (a \cdot b)^2$$

$$(a_i \delta_j \wedge b_j \delta_j) \cdot (a_i \delta_j \wedge b_j \delta_j) + (a_i \delta_i \cdot b_j \delta_j)^2$$

$$= (a_i b_j \varepsilon_{ijk} \delta_k) \cdot (a_i b_j \varepsilon_{ijk} \delta_k) + (a_i b_j \delta_{ij})^2$$

$$= (a_i b_j)^2 \varepsilon_{ijk} \varepsilon_{kij} (\delta_k \cdot \delta_k) + (a_i b_i)^2$$

$$= (a_i b_j)^2 [\delta_{ii} \delta_{jj} - \delta_{ij} \delta_{ji}] + (a_i b_i)^2$$

$$= (a_i b_j)^2 - \cancel{(a_i b_i)^2} + \cancel{(a_i b_i)^2}$$

$$= (a_i b_j)^2$$

$$\begin{aligned}
 (a \wedge b)^2 &= \left(\sum_{ijk} \epsilon_{ijk} a_j b_k \right)^2 \\
 &= \epsilon_{ijk} a_j b_k \epsilon_{imn} a_m b_n \\
 &= a_i^2 b_j^2.
 \end{aligned}$$

$$\begin{aligned}
 (a \wedge b) \wedge (a \wedge b) &= \epsilon_{ijk} a_i b_j \delta_k \wedge \epsilon_{pqr} a_p b_q \delta_r \\
 &= \epsilon_{ijk} a_i b_j \epsilon_{pqr} a_p b_q \epsilon_{lkr} \delta_l \\
 &= \epsilon_{ijk} a_i b_j a_p b_q \epsilon_{pqr} \epsilon_{rkl} \delta_l \\
 &= \epsilon_{ijk} a_i b_j a_p b_q \{ \delta_{pr} \delta_{qk} - \delta_{pk} \delta_{qr} \} \delta_l \\
 &= \epsilon_{ijq} a_i b_j a_l b_q \delta_l - \epsilon_{ijp} a_i b_j a_p b_l \delta_l \\
 &= a_l [b_l \cdot (a \wedge b)] - b_l [a_l \cdot (a \wedge b)] \\
 &= a_l [a_l \cdot (\cancel{b \wedge b})] - b_l [b_l \cdot (\cancel{a \wedge a})] \\
 &= \underline{\underline{0}}
 \end{aligned}$$

$$4) \quad A : B = A_{ij} \underline{\delta_i} \underline{\delta_j} : B_{p2} \underline{\delta_p} \underline{\delta_2}$$

$$= A_{ij} B_{p2} (\underline{\delta_j} \cdot \underline{\delta_p}) (\underline{\delta_i} \cdot \underline{\delta_2})$$

$$= A_{ij} B_{ji}$$

$$\underline{\delta} = \begin{bmatrix} 1 & 0 & 0 \\ 0 & 1 & 0 \\ 0 & 0 & 1 \end{bmatrix}$$

$$\underline{\delta} : \underline{\delta} = \delta_{ij} \underline{\delta_i} \underline{\delta_j} : \delta_{p2} \underline{\delta_p} \underline{\delta_2} \quad \Rightarrow$$

$$= \delta_{ij} \delta_{p2} (\underline{\delta_j} \cdot \underline{\delta_p}) (\underline{\delta_i} \cdot \underline{\delta_2})$$

$$= \delta_{ij} \delta_{ji} = \underline{\underline{\delta_{ii}}} = \underline{\underline{1+1+1=3}}$$

(keeping $i=j$ using one of the δ_{ij})

$$\underline{\nabla} \cdot \underline{v} = \frac{\partial}{\partial x_i} \underline{\delta_i} \cdot (\omega_k r_p \varepsilon_{jkp} \underline{\delta_j})$$

$$= \frac{\partial}{\partial x_i} (\omega_k r_p \varepsilon_{ikp}) = \omega_k \varepsilon_{ikp} \frac{\partial r_p}{\partial x_i}$$

$$= \omega_k \varepsilon_{iki} = 0$$

